src/QueryConformance.v
@@ -17,13 +17,30 @@ Require Import SchemaWellFormedness.
 Section QueryConformance.
 
   Variables Name Vals : ordType.
-  Variable sch : @schema Name.
   
-  Implicit Type schema : @wfSchema Name Vals sch.  
+  Implicit Type schema : @wfSchema Name Vals.  
   Implicit Type queries : seq (@Query Name Vals).
   Implicit Type query : @Query Name Vals.
   Implicit Type type : @type Name.
 
+
+  
+  Lemma fset1I_eq {A : ordType} (a b : A) :
+    (fset1 a :&: fset1 b)%fset != fset0 -> a = b.
+  Proof.
+    rewrite fset1I.
+    case: ifP => //.
+    by move/fset1P => //.
+  Qed.
+
+  Lemma fset1I_N_fset0 {A : ordType} (a : A) :
+    (fset1 a :&: fset1 a)%fset != fset0.
+  Proof.
+    rewrite fset1I.
+    case: ifP => //.
+      by rewrite in_fset1 eqxx.
+  Qed.
+  
   (** Checks whether a query's argument (arg name + value associated) conforms to an argument
       of a field defined in the schema.
       
@@ -74,24 +91,36 @@ Section QueryConformance.
      ty \in implementation schema parent_type |
      ty \in union_members schema parent_type].
   Proof.
-    move/is_object_type_E=> [obj [intfs [flds Hlook]]].
+    case: schema=> sch Hty Hwf Hobj Hspread.
+    apply/in_possible_typesPwf=> //.
+    move: Hspread.
     rewrite /is_fragment_spread_possible.
-    rewrite {1}/get_possible_types Hlook fset1I.
-    case: ifP => //.
-      by move/in_possible_types_E.
+    rewrite /get_possible_types.
+    move/is_object_type_wfP: Hobj => [intfs [flds Hlook]].
+    rewrite Hlook.
+    case lookup_type; case.
+    - by move=> _; rewrite fsetI0.
+    - by move=> _ _ _ /fset1I_eq ->; rewrite in_fset1.
+    - by move=> i ifldsc; rewrite fset1I; case: ifP => //.
+    - by move=> u mbs; rewrite fset1I; case: ifP.
+    - by move=> e ev; rewrite fsetI0.
+    - by rewrite fsetI0.
   Qed.
 
-  Lemma eq_spreads schema ty :
+
+  (*Lemma eq_spreads schema ty :
     [\/ is_object_type schema ty, is_interface_type schema ty | is_union_type schema ty] ->
     is_fragment_spread_possible schema ty ty.
   Proof.
     case.
-    move/is_object_type_E=> [obj [intf [flds Hlook]]].
-    rewrite /is_fragment_spread_possible /get_possible_types Hlook.
-    rewrite fset1I /= inE.
-    case: ifP=> //. case: eqP => //.
-  Admitted.
+    - move/is_object_type_E=> [obj [intf [flds Hlook]]].
+      rewrite /is_fragment_spread_possible /get_possible_types Hlook.
+        by apply: fset1I_N_fset0.
+    - move/is_interface_type_E => [intf [flds Hlook]].
+      rewrite /is_fragment_spread_possible /get_possible_types Hlook.
+   *)
 
+      
   (** Checks whether a query conforms to a given schema.
       
       Every query (or selection of fields) is set in a given context
@@ -133,7 +162,7 @@ Section QueryConformance.
         end
         
     | InlineFragment t ϕ =>
-      [&& [|| is_object_type schema t, is_interface_type schema t | is_union_type schema t],
+      [&& [|| is_object_type schema t, is_interface_type schema t | is_union_type schema t], (* This might be a bit redundant *)
        is_fragment_spread_possible schema ty t,
        ϕ != [::] &
        all (query_conforms schema t) ϕ]
@@ -141,10 +170,11 @@ Section QueryConformance.
 
   Definition queries_conform schema ty queries := (queries != [::]) && (all (query_conforms schema ty) queries).
 
-  Lemma queries_conformE schema ty queries :
+ (* Lemma queries_conformE schema ty queries :
     queries_conform schema ty queries ->
     queries != [::] /\ all (query_conforms schema ty) queries.
   Proof. by rewrite /queries_conform; move/andP. Qed.
+  *)
   
   Lemma ty_not_scalar_or_enum schema ty tdef:
     lookup_type schema ty = Some tdef ->
@@ -162,14 +192,8 @@ Section QueryConformance.
   Qed.
 
 
-  Lemma fset1I_N_fset0 {A : ordType} (a b : A) :
-    (fset1 a :&: fset1 b)%fset != fset0 -> a = b.
-  Proof.
-    rewrite fset1I.
-    case: ifP => //.
-    move/fset1P => //.
-  Qed.
 
+  Ltac wfquery := case: schema=> sch Hhasty Hwf.
  
   Lemma object_spreads_in_object_scope schema type_in_scope t ϕ :
     is_object_type schema type_in_scope ->
@@ -178,6 +202,7 @@ Section QueryConformance.
     query_conforms schema type_in_scope (InlineFragment t ϕ) <->
     t = type_in_scope.
   Proof.
+    wfquery.
     move=> Hobj'.
     pose H' := Hobj'.
     move/is_object_type_E: H' => [obj [intfs [flds H]]].
@@ -187,14 +212,19 @@ Section QueryConformance.
     - rewrite /query_conforms.
       move/and4P=> [/or3P _ Hspread _ _].
       move: (object_spreads_E Hobj Hspread)=> [||] //.
-        rewrite /implementation.
-      by rewrite /union_members H.
+      * move/has_implementation_is_interface=> Hcontr.
+        move: (is_object_type_interfaceN Hobj') => //.
+          by rewrite Hcontr.
+      * move/in_union => Hcontr.
+        move: (is_object_type_unionN Hobj').
+          by rewrite Hcontr.
     - move=> Heq; rewrite Heq /=.
       move: Hqsc; rewrite /queries_conform.
       move/andP=> [Hne Hall].
       apply/and4P; split=> //.
         by apply/or3P; constructor 1.
-        by apply: eq_spreads; constructor 1.
+        rewrite /is_fragment_spread_possible /get_possible_types.
+        by rewrite H; apply: fset1I_N_fset0.
       by rewrite Heq in Hall.
   Qed.
 
@@ -204,14 +234,12 @@ Section QueryConformance.
     query_conforms schema type_in_scope (InlineFragment t ϕ) ->
     type_in_scope \in implementation schema t.
   Proof.
-    funelim (is_object_type schema type_in_scope) => // _.
-    funelim (is_interface_type schema t) => // _.
-    rewrite /query_conforms.
-    move/and4P=> [_ Hspread _ _].
-    move: Hspread; rewrite /is_fragment_spread_possible /get_possible_types Heq Heq0.
+    move/is_object_type_wfP=> [intfs [flds Hlook]].
+    move/is_interface_type_wfP=> [iflds Hlook'].
+    rewrite /query_conforms=> /and4P [_ Hspread _ _].
+    move: Hspread; rewrite /is_fragment_spread_possible /get_possible_types Hlook Hlook'.
     rewrite fsetIC fset1I.
-    case: ifP => //.
-      by rewrite /implementation Heq in_fset.
+    by case: ifP.
   Qed.
 
   Lemma union_spreads_in_object_scope schema type_in_scope t ϕ :
@@ -227,49 +255,81 @@ Section QueryConformance.
     move: Hspread; rewrite /is_fragment_spread_possible /get_possible_types Heq Heq0.
     rewrite fsetIC fset1I.
     case: ifP => //.
-    by rewrite /union_members Heq in_fset.
+    by rewrite /union_members Heq.
   Qed.
 
   Lemma abstract_spreads_in_object_scope schema type_in_scope t ϕ :
     is_object_type schema type_in_scope ->
     queries_conform schema t ϕ ->
     (is_interface_type schema t \/ is_union_type schema t) ->
-    query_conforms schema type_in_scope (InlineFragment t ϕ) <->
-    (type_in_scope \in implementation schema t \/ type_in_scope \in union_members schema t).
+    reflect (type_in_scope \in implementation schema t \/ type_in_scope \in union_members schema t)
+            (query_conforms schema type_in_scope (InlineFragment t ϕ)).
   Proof.
     move=> Hobj Hqsc Htype.
-    split.
+    apply: (iffP idP).
     - case: Htype => [Hint | Hunion].
         by move/(interface_spreads_in_object_scope Hobj Hint); left.
       by move/(union_spreads_in_object_scope Hobj Hunion); right.
-    - move: Hqsc; rewrite /queries_conform; move/andP=> [Hne Hall].
+    - move: Hqsc; rewrite /queries_conform => /andP [Hne Hall].
       move=> H.      
       rewrite /query_conforms; apply/and4P; split=> //.
-      apply/or3P.
-      by case: Htype; [constructor 2 | constructor 3].
-      rewrite /is_fragment_spread_possible.
-      Admitted.
+      * by apply/or3P; case: Htype; [constructor 2 | constructor 3].
+      * move/is_object_type_wfP: Hobj => [intfs [flds Holook]].
+        case: H => [Himpl | Hmb]; 
+        rewrite /is_fragment_spread_possible /get_possible_types.
+        move: (has_implementation_is_interface Himpl) => /is_interface_type_wfP [iflds Hilook].
+        by rewrite Holook Hilook fsetIC fset1I Himpl.
+        move: (in_union Hmb) => /is_union_type_wfP [mbs Hulook].
+        rewrite Holook Hulook fsetIC fset1I.
+        rewrite /union_members Hulook in Hmb.
+        by rewrite Hmb.
+  Qed.
 
-      
-  Lemma object_spreads_in_interface_scope schema type_in_scope t ϕ :
-    is_object_type schema t ->
-    is_interface_type schema type_in_scope ->
-    queries_conform schema t ϕ ->
-    query_conforms schema type_in_scope (InlineFragment t ϕ) <->
-    t \in implementation schema type_in_scope.
-  Proof.
-  Admitted.
+  Ltac query_conforms := rewrite /query_conforms -/(query_conforms _ _); try move/and4P; try apply/and4P.
+
 
 
 
   
-  Lemma nested_field_obj_int_union schema ty n α ϕ :
-    query_conforms schema ty (NestedField n α ϕ) ->
-    is_object_type schema n \/ is_interface_type schema n \/ is_union_type schema n.
+  
+  Lemma object_spreads_in_interface_scope schema type_in_scope t ϕ :
+    is_object_type schema t ->
+    is_interface_type schema type_in_scope ->
+    queries_conform schema t ϕ ->
+    reflect (t \in implementation schema type_in_scope)
+            (query_conforms schema type_in_scope (InlineFragment t ϕ)).
   Proof.
-  Admitted.
+    move=> Hobj Hintf Hqsc.
+    apply: (iffP idP).
+    - query_conforms.
+      move=> [_ Hspread _ _].
+      move: (object_spreads_E Hobj Hspread) => [Heq | // | /in_union Hun].
+      * move: (is_object_type_interfaceN Hobj); rewrite Heq.
+        by rewrite /negb Hintf.
+      * by move: (is_interface_type_unionN Hintf); rewrite /negb Hun.
+    - move=> Himpl.
+      query_conforms; split.
+      * by apply/or3P; constructor 1.
+      * rewrite /is_fragment_spread_possible.
+        move/get_possible_types_interfaceE: Hintf => ->.
+        move/get_possible_types_objectE: Hobj => ->.
+        by rewrite fset1I Himpl.
+      * by move: Hqsc; rewrite /queries_conform => /andP [H _].
+      * by move: Hqsc; rewrite /queries_conform => /andP [_ H].
+  Qed.
+        
+  Lemma nested_field_is_obj_or_abstract schema ty n α ϕ :
+    query_conforms schema ty (NestedField n α ϕ) ->
+    is_object_type schema ty \/ is_interface_type schema ty.
+  Proof.
+    rewrite /query_conforms.
+    case Hlook: lookup_field_in_type => [fld|] // _.
+    have H: lookup_field_in_type schema ty n by rewrite /isSome Hlook.
+      by apply: (lookup_field_in_type_is_obj_or_intf H).
+  Qed.
 
-  Definition is_inline_fragment := @is_inline_fragment Name Vals.
+
+  Notation is_inline_fragment := (@is_inline_fragment Name Vals).
 
 
     
@@ -284,48 +344,8 @@ Section QueryConformance.
     case Hlookf : lookup_field_in_type => [fld|] //.
   Abort.
 
-  Lemma lookup_field_object_or_interface schema ty fname fld :
-    lookup_field_in_type schema ty fname = Some fld ->
-    is_object_type schema ty \/ is_interface_type schema ty.
-  Proof.
-    rewrite /lookup_field_in_type /fields.
-    case Hlook: lookup_type => [tdef|] //.
-    case: tdef Hlook => // [o intfs flds | i flds] Hlook _.
-    by left; rewrite /is_object_type Hlook.
-    by right; rewrite /is_interface_type Hlook.
-  Qed.
+  
 
-  Lemma has_implementation_is_interface schema ty ty' :
-    ty' \in implementation schema ty ->
-            is_interface_type schema ty.
-  Proof.
-    rewrite /implementation.
-    case Hlook: lookup_type => [tdef|] //.
-    case: tdef Hlook => // i flds Hlook _.
-      by rewrite /is_interface_type Hlook.
-  Qed.
-
-  Lemma in_implementation_is_object schema ty :
-    forall ty', ty' \in implementation schema ty ->
-                   is_object_type schema ty'.
-    Admitted.
-
-  Lemma has_members_is_union schema ty ty' :
-    ty' \in union_members schema ty ->
-            is_union_type schema ty.
-  Proof.
-    rewrite /union_members.
-    case Hlook: lookup_type => [tdef|] //.
-    case: tdef Hlook => // i flds Hlook _.
-      by rewrite /is_union_type Hlook.
-  Qed.
-
-  Lemma in_union_is_object schema ty :
-    forall ty',
-      ty' \in union_members schema ty ->
-              is_object_type schema ty'.
-  Proof.
-    Admitted.
             
     
   Lemma type_in_scope_N_scalar_enum schema type_in_scope ϕ :
@@ -334,40 +354,19 @@ Section QueryConformance.
      is_interface_type schema type_in_scope |
      is_union_type schema type_in_scope].
   Proof.
-    case: ϕ.
-    - move=> f α.
-      rewrite /query_conforms.
-      case Hlook: lookup_field_in_type => [fld|] // _.
-      move: (lookup_field_object_or_interface Hlook) => [Hobj | Hint].
-        by constructor 1.
-        by constructor 2.
-    - move=> l f α.
-      rewrite /query_conforms.
-      case Hlook: lookup_field_in_type => [fld|] // _.
-      move: (lookup_field_object_or_interface Hlook) => [Hobj | Hint].
-        by constructor 1.
-        by constructor 2.
-    - move=> f α ϕ.
-      rewrite /query_conforms.
-      case Hlook: lookup_field_in_type => [fld|] // _.
-      move: (lookup_field_object_or_interface Hlook) => [Hobj | Hint].
-        by constructor 1.
-        by constructor 2.
-    - move=> l f α ϕ.
-      rewrite /query_conforms.
-      case Hlook: lookup_field_in_type => [fld|] // _.
-      move: (lookup_field_object_or_interface Hlook) => [Hobj | Hint].
-        by constructor 1.
-        by constructor 2.
-    - move=> t ϕ.
-      rewrite /query_conforms.
-      move/and4P=> [/or3P Hty Hspread Hne _] => //.
-      move: Hspread.
-      rewrite /is_fragment_spread_possible.
-      rewrite /get_possible_types fsetIC.
-      case Hlook: lookup_type => [tdef|] //.
-      case: tdef Hlook => //; do ?[rewrite fset0I //=].
-      move=> obj intfs flds Hlook _.
+    case: ϕ; [move=> f α | move=> l f α | move=> f α ϕ | move=> l f α ϕ | move=> t ϕ];
+    do ?[rewrite /query_conforms;
+         case Hlook: lookup_field_in_type => [fld|] // _;
+         have H: lookup_field_in_type schema type_in_scope f by rewrite /isSome Hlook].
+    all: do ?[by move: (lookup_field_in_type_is_obj_or_intf H) => [Hobj | Hint]; [constructor 1 | constructor 2]].
+
+    move/and4P=> [/or3P Hty Hspread Hne _] => //.
+    move: Hspread.
+    rewrite /is_fragment_spread_possible.
+    rewrite /get_possible_types fsetIC.
+    case Hlook: lookup_type => [tdef|] //.
+    case: tdef Hlook => //; do ?[rewrite fset0I //=].
+    move=> obj intfs flds Hlook _.
       by constructor 1; rewrite /is_object_type Hlook /=.
       move=> i flds Hlook _.
         by constructor 2; rewrite /is_interface_type Hlook /=.
@@ -386,7 +385,7 @@ Section QueryConformance.
     rewrite /queries_conform.
     case: ϕ => // hd tl.
     move/andP=> [Hnil /= /andP [Hhd _]].
-    apply: (type_in_scope_N_scalar_enum Hhd).
+    by apply: (type_in_scope_N_scalar_enum Hhd).
   Qed.
 
   
@@ -437,6 +436,7 @@ Section QueryConformance.
      do ? case lookup_field_in_type => //.
     - Admitted. (* Invalid case - all fields *)
 
+  (* Not valid 
   Lemma inline_conforms_to_same_type schema t ϕ :
     [\/ is_object_type schema t, is_interface_type schema t | is_union_type schema t] ->
     queries_conform schema t ϕ ->
@@ -444,7 +444,9 @@ Section QueryConformance.
   Proof.
     move=> Hty Hqsc /=; apply/and3P; split=> //.
     by apply/or3P.
-    by apply: eq_spreads.
-  Qed.
+    case: Hty => [Hobj | Hintf | Hunion]; rewrite /is_fragment_spread_possible;
+    [rewrite (get_possible_types_objectE Hobj) | rewrite (get_possible_types_interfaceE Hintf)|  ]. apply: fset1I_N_fset0.
+      by apply: eq_spreads.
+  Qed. *)
   
 End QueryConformance.
